coq_translation/axiomatized/examples/functions/functions_order.v
@@ -27,18 +27,133 @@ Module OtherType.
 End OtherType.
 Definition OtherType := @OtherType.t.
 
+Module Impl_functions_order_SomeType.
+  Definition Self := functions_order.SomeType.
+  
+  Parameter meth2 : forall `{H' : State.Trait}, Self -> M (H := H') unit.
+  
+  Global Instance Method_meth2 `{H' : State.Trait} : Notation.Dot "meth2" := {
+    Notation.dot := meth2;
+  }.
+  
+  Parameter meth1 : forall `{H' : State.Trait}, Self -> M (H := H') unit.
+  
+  Global Instance Method_meth1 `{H' : State.Trait} : Notation.Dot "meth1" := {
+    Notation.dot := meth1;
+  }.
+End Impl_functions_order_SomeType.
+
+Module SomeTrait.
+  Class Trait (Self : Set) : Type := {
+    some_trait_foo `{H' : State.Trait} : (ref Self) -> M (H := H') unit;
+    some_trait_bar `{H' : State.Trait} : (ref Self) -> M (H := H') unit;
+  }.
+  
+  Global Instance Method_some_trait_foo `{H' : State.Trait} `(Trait)
+    : Notation.Dot "some_trait_foo" := {
+    Notation.dot := some_trait_foo;
+  }.
+  Global Instance Method_some_trait_bar `{H' : State.Trait} `(Trait)
+    : Notation.Dot "some_trait_bar" := {
+    Notation.dot := some_trait_bar;
+  }.
+End SomeTrait.
+
+Module Impl_functions_order_SomeTrait_for_functions_order_SomeType.
+  Definition Self := functions_order.SomeType.
+  
+  Parameter some_trait_bar :
+      forall `{H' : State.Trait},
+      (ref Self) -> M (H := H') unit.
+  
+  Global Instance Method_some_trait_bar `{H' : State.Trait} :
+    Notation.Dot "some_trait_bar" := {
+    Notation.dot := some_trait_bar;
+  }.
+  
+  Parameter some_trait_foo :
+      forall `{H' : State.Trait},
+      (ref Self) -> M (H := H') unit.
+  
+  Global Instance Method_some_trait_foo `{H' : State.Trait} :
+    Notation.Dot "some_trait_foo" := {
+    Notation.dot := some_trait_foo;
+  }.
+  
+  Global Instance I : functions_order.SomeTrait.Trait Self := {
+    functions_order.SomeTrait.some_trait_bar `{H' : State.Trait}
+      :=
+      some_trait_bar;
+    functions_order.SomeTrait.some_trait_foo `{H' : State.Trait}
+      :=
+      some_trait_foo;
+  }.
+  Global Hint Resolve I : core.
+End Impl_functions_order_SomeTrait_for_functions_order_SomeType.
+
+Module Impl_functions_order_SomeTrait_for_functions_order_OtherType.
+  Definition Self := functions_order.OtherType.
+  
+  Parameter some_trait_foo :
+      forall `{H' : State.Trait},
+      (ref Self) -> M (H := H') unit.
+  
+  Global Instance Method_some_trait_foo `{H' : State.Trait} :
+    Notation.Dot "some_trait_foo" := {
+    Notation.dot := some_trait_foo;
+  }.
+  
+  Parameter some_trait_bar :
+      forall `{H' : State.Trait},
+      (ref Self) -> M (H := H') unit.
+  
+  Global Instance Method_some_trait_bar `{H' : State.Trait} :
+    Notation.Dot "some_trait_bar" := {
+    Notation.dot := some_trait_bar;
+  }.
+  
+  Global Instance I : functions_order.SomeTrait.Trait Self := {
+    functions_order.SomeTrait.some_trait_foo `{H' : State.Trait}
+      :=
+      some_trait_foo;
+    functions_order.SomeTrait.some_trait_bar `{H' : State.Trait}
+      :=
+      some_trait_bar;
+  }.
+  Global Hint Resolve I : core.
+End Impl_functions_order_SomeTrait_for_functions_order_OtherType.
+
+Parameter depends_on_trait_impl :
+    forall `{H' : State.Trait},
+    u32 -> bool -> M (H := H') unit.
+
 Module inner_mod.
+  Parameter tar : forall `{H' : State.Trait}, M (H := H') unit.
+  
   Parameter bar : forall `{H' : State.Trait}, M (H := H') unit.
   
   Module nested_mod.
+    Parameter tack : forall `{H' : State.Trait}, M (H := H') unit.
+    
     Parameter tick : forall `{H' : State.Trait}, M (H := H') unit.
   End nested_mod.
 End inner_mod.
 
 Parameter bar : forall `{H' : State.Trait}, M (H := H') unit.
 
+Parameter tar : forall `{H' : State.Trait}, M (H := H') unit.
+
 Module nested_mod.
+  Parameter tack : forall `{H' : State.Trait}, M (H := H') unit.
+  
   Parameter tick : forall `{H' : State.Trait}, M (H := H') unit.
 End nested_mod.
 
 Parameter tick : forall `{H' : State.Trait}, M (H := H') unit.
+
+Parameter tack : forall `{H' : State.Trait}, M (H := H') unit.
+
+Parameter foo : forall `{H' : State.Trait}, M (H := H') unit.
+
+(* #[allow(dead_code)] - function was ignored by the compiler *)
+Parameter main : forall `{H' : State.Trait}, M (H := H') unit.
