coq_translation/axiomatized/examples/modules/struct_visibility.v
@@ -39,6 +39,19 @@ Module my.
     End ClosedBox.
   End ClosedBox.
   Definition ClosedBox (T : Set) : Set := ClosedBox.t (T := T).
+  
+  Module Impl_struct_visibility_my_ClosedBox_T.
+    Definition Self := struct_visibility.my.ClosedBox T.
+    
+    Parameter new :
+        forall `{H' : State.Trait},
+        T -> M (H := H') (struct_visibility.my.ClosedBox T).
+    
+    Global Instance AssociatedFunction_new `{H' : State.Trait} :
+      Notation.DoubleColon Self "new" := {
+      Notation.double_colon := new;
+    }.
+  End Impl_struct_visibility_my_ClosedBox_T.
 End my.
 
 Module OpenBox.
@@ -78,3 +91,19 @@ Module ClosedBox.
   End ClosedBox.
 End ClosedBox.
 Definition ClosedBox (T : Set) : Set := ClosedBox.t (T := T).
+
+Module Impl_struct_visibility_my_ClosedBox_T_2.
+  Definition Self := struct_visibility.my.ClosedBox T.
+  
+  Parameter new :
+      forall `{H' : State.Trait},
+      T -> M (H := H') (struct_visibility.my.ClosedBox T).
+  
+  Global Instance AssociatedFunction_new `{H' : State.Trait} :
+    Notation.DoubleColon Self "new" := {
+    Notation.double_colon := new;
+  }.
+End Impl_struct_visibility_my_ClosedBox_T_2.
+
+(* #[allow(dead_code)] - function was ignored by the compiler *)
+Parameter main : forall `{H' : State.Trait}, M (H := H') unit.
