coq_translation/axiomatized/examples/testing/unit_testing.v
@@ -2,3 +2,16 @@
 Require Import CoqOfRust.CoqOfRust.
 
 Parameter add : forall `{H' : State.Trait}, i32 -> i32 -> M (H := H') i32.
+
+(* #[allow(dead_code)] - function was ignored by the compiler *)
+Parameter bad_add : forall `{H' : State.Trait}, i32 -> i32 -> M (H := H') i32.
+
+Module tests.
+  Parameter test_add : forall `{H' : State.Trait}, M (H := H') unit.
+  
+  Parameter test_bad_add : forall `{H' : State.Trait}, M (H := H') unit.
+End tests.
+
+Parameter test_add : forall `{H' : State.Trait}, M (H := H') unit.
+
+Parameter test_bad_add : forall `{H' : State.Trait}, M (H := H') unit.
